src/SDK/Keyring/KMSKeyring.dfy
@@ -25,7 +25,7 @@ module {:extern "KMSKeyringDef"} KMSKeyringDef {
 
   class KMSKeyring extends KeyringDefs.Keyring {
 
-    const clientSupplier: KMSUtils.KMSClientSupplier
+    const clientSupplier: KMSUtils.AWSKMSClientSupplier
     const keyIDs: seq<KMSUtils.CustomerMasterKey>
     const generator: Option<KMSUtils.CustomerMasterKey>
     const grantTokens: seq<KMSUtils.GrantToken>
@@ -41,7 +41,7 @@ module {:extern "KMSKeyringDef"} KMSKeyringDef {
       && (clientSupplier in Repr && clientSupplier.Repr <= Repr && this !in clientSupplier.Repr && clientSupplier.Valid())
     }
 
-    constructor (clientSupplier: KMSUtils.KMSClientSupplier, keyIDs: seq<KMSUtils.CustomerMasterKey>, generator: Option<KMSUtils.CustomerMasterKey>, grantTokens: seq<KMSUtils.GrantToken>)
+    constructor (clientSupplier: KMSUtils.AWSKMSClientSupplier, keyIDs: seq<KMSUtils.CustomerMasterKey>, generator: Option<KMSUtils.CustomerMasterKey>, grantTokens: seq<KMSUtils.GrantToken>)
       requires clientSupplier.Valid()
       requires 0 <= |grantTokens| <= KMSUtils.MAX_GRANT_TOKENS
       ensures this.clientSupplier == clientSupplier
@@ -205,8 +205,8 @@ module {:extern "KMSKeyringDef"} KMSKeyringDef {
           var regionRes := RegionFromKMSKeyARN(providerInfo.value);
           var regionOpt := regionRes.ToOption();
           var clientRes := clientSupplier.GetClient(regionOpt);
-          if clientRes.KMSClientSuccess? {
-            var client := clientRes.Extract();
+          if clientRes.Success? {
+            var client := clientRes.value;
             var decryptResponseResult := client.Decrypt(decryptRequest);
             if decryptResponseResult.Success? {
               var decryptResponse := decryptResponseResult.value;
